Towards proving function expressions.

LambdaS5/coq/EjsSyntax.v
@@ -62,3 +62,5 @@ with switchbody : Type :=
 .
 
 Definition expr_seqs es := fold_left (fun e1 e2 => expr_seq e2 e1) expr_empty es.
+
+Definition prog_strictness p := match p with prog_intro b _ _ => b end.
